Prove BreakConstAssigns correct
Required adding a not-strictly-necessary sortedness check
Originally *fully* AI generated, manually reworked

vera/BreakConstAssigns.v
@@ -4,8 +4,10 @@ From vera Require Import Decidable.
 From vera Require Import Tactics.
 From vera Require Import Bitvector.
 From vera Require Import Common.
+From vera Require Import VerilogSemantics.
 Import Verilog.
-(* From vera Require VerilogSemantics. *)
+Import ExactEquivalence.
+Import CombinationalOnly.
 
 From ExtLib Require Import Structures.Monads.
 From ExtLib Require Import Programming.Show.
@@ -29,88 +31,141 @@ Import EqNotations.
 Import SigTNotations.
 Opaque N.add N.sub.
 
-Equations break_const_assign {w} (t : assign_target w) : assign_target_wf t -> XBV.xbv w -> list module_item := {
-  | (@AssignConcat w_hi w_lo target_hi target_lo), wf, val :=
-    break_const_assign target_hi _ (XBV.extr val w_lo w_hi)
-    ++ break_const_assign target_lo _ (XBV.extr val 0 w_lo)
-  | target, t_wf, val := [AlwaysComb (BlockingAssign target t_wf (IntegerLiteral _ val))]
-}.
-Next Obligation. inv wf. assumption. Qed.
-Next Obligation. inv wf. assumption. Qed.
+Section definition.
+  Equations break_const_assign {w} (t : assign_target w) : assign_target_wf t -> XBV.xbv w -> list module_item := {
+    | (@AssignConcat w_hi w_lo target_hi target_lo), wf, val :=
+      break_const_assign target_lo _ (XBV.extr val 0 w_lo)
+      ++ break_const_assign target_hi _ (XBV.extr val w_lo w_hi)
+    | target, t_wf, val := [AlwaysComb (BlockingAssign target t_wf (IntegerLiteral _ val))]
+  }.
+  Next Obligation. inv wf. assumption. Qed.
+  Next Obligation. inv wf. assumption. Qed.
 
-Equations break_const_assigns_module_item : module_item -> list module_item := {
-  | AlwaysComb (BlockingAssign target wf (IntegerLiteral _ val)) :=
-    trace
-      ("Break const assign to " ++ to_string target)
-      (break_const_assign target wf val)
-  | mi := [ mi ]
-}.
+  Equations break_const_assigns_module_body : list module_item -> list module_item := {
+    | AlwaysComb (BlockingAssign target wf (IntegerLiteral _ val)) :: tl =>
+      trace
+        ("Break const assign to " ++ to_string target)
+        (break_const_assign target wf val)
+      ++ break_const_assigns_module_body tl
+    | mi :: tl => mi :: break_const_assigns_module_body tl
+    | [] => []
+  }.
 
-Definition break_const_assigns_module_body : list module_item -> list module_item :=
-  flat_map break_const_assigns_module_item.
+  Definition break_const_assigns_vmodule {i o} (v : vmodule i o) : string + vmodule i o :=
+    traceBracket ("Break const assigns " ++ Verilog.modName v) (
+      assert_dec (vmodule_sorted v) "Unsorted module in break_const_assigns";;
+      ret {|
+        modName := modName v;
+        modBody := break_const_assigns_module_body (modBody v);
+        modWfIODisjoint := modWfIODisjoint v;
+        modWfInputsNoDup := modWfInputsNoDup v;
+        modWfOutputsNoDup := modWfOutputsNoDup v;
+      |}).
+End definition.
 
-Definition break_const_assigns_vmodule {i o} (v : vmodule i o) : vmodule i o :=
-  traceBracket ("Break const assigns " ++ Verilog.modName v) {|
-    modName := modName v;
-    modBody := break_const_assigns_module_body (modBody v);
-    modWfIODisjoint := modWfIODisjoint v;
-    modWfInputsNoDup := modWfInputsNoDup v;
-    modWfOutputsNoDup := modWfOutputsNoDup v;
-  |}.
+Section accessed.
+  Lemma break_const_assign_writes {w} (target : assign_target w) wf val :
+    LocationSet.Equal
+      (module_body_writes (break_const_assign target wf val))
+      (assign_target_writes target).
+  Proof.
+    funelim (break_const_assign target wf val).
+    all: simpl.
+    all: try LocationSet.setdec; expect 1.
+    rewrite module_body_writes_app, H, H0.
+    LocationSet.setdec.
+  Qed.
+End accessed.
 
-Lemma break_const_assigns_module_item_writes mi :
-  LocationSet.Equal
-    (module_body_writes (break_const_assigns_module_item mi))
-    (module_item_writes mi).
+Section semantics.
+  Lemma exec_module_body_app regs body1 body2 :
+    exec_module_body regs (body1 ++ body2) =
+    exec_module_body (exec_module_body regs body1) body2.
+  Proof.
+    revert regs.
+    induction body1; intros regs; simpl; simp exec_module_body; simpl.
+    - reflexivity.
+    - apply IHbody1.
+  Qed.
+
+  Lemma exec_break_const_assign {w} (target : assign_target w) wf val regs :
+    exec_module_body regs (break_const_assign target wf val) =
+    set_target regs target val.
+  Proof.
+    funelim (break_const_assign target wf val).
+    all: simp exec_module_body exec_module_item exec_statement eval_expr set_target; simpl.
+    all: try reflexivity. all: expect 1.
+    rewrite exec_module_body_app, H, H0.
+    reflexivity.
+  Qed.
+
+  Lemma exec_break_const_assigns_module_body regs body :
+    exec_module_body regs (break_const_assigns_module_body body) =
+    exec_module_body regs body.
+  Proof.
+    funelim (break_const_assigns_module_body body).
+    all: clear Heqcall.
+    all: simp exec_module_body; simpl.
+    all: try reflexivity; try eauto.
+    rename_match (forall regs, exec_module_body regs _ = _) into IH.
+    rewrite exec_module_body_app, exec_break_const_assign, IH.
+    reflexivity.
+  Qed.
+End semantics.
+
+Section sort.
+  #[local]
+  Lemma break_const_assign_sorted {w} (target : assign_target w) wf val vars :
+    LocationSet.Disjoint (assign_target_writes target) vars ->
+    module_items_sorted vars (break_const_assign target wf val).
+  Proof.
+    funelim (break_const_assign target wf val).
+    all: intros Hdisjoint; simpl in *.
+    all: try (constructor; [LocationSet.setdec | exact Hdisjoint | constructor]);
+      expect 1.
+    apply module_items_sorted_app.
+    - apply H. LocationSet.setdec.
+    - apply H0. rewrite break_const_assign_writes.
+      pose proof wf as Hwf. inv Hwf.
+      LocationSet.setdec.
+  Qed.
+
+  Lemma break_const_assigns_sorted vars body :
+    module_items_sorted vars body ->
+    module_items_sorted vars (break_const_assigns_module_body body).
+  Proof.
+    funelim (break_const_assigns_module_body body).
+    all: clear Heqcall; intros Hsorted; inv Hsorted.
+    all: simpl.
+    all: try (constructor; try assumption; eauto).
+    rename_match (forall vars, module_items_sorted vars tl -> _) into IH.
+    rename_match (LocationSet.Disjoint _ vars) into Hdisjoint.
+    rename_match (module_items_sorted _ tl) into Hsorted_tl.
+    apply module_items_sorted_app.
+    - apply break_const_assign_sorted. exact Hdisjoint.
+    - apply IH.
+      eapply module_items_sorted_permute_vars with
+        (l := assign_target_writes target ∪ vars).
+      + rewrite break_const_assign_writes. LocationSet.setdec.
+      + exact Hsorted_tl.
+  Qed.
+End sort.
+
+Theorem break_const_assigns_exact_equivalence {i o} (v1 v2 : vmodule i o) :
+  break_const_assigns_vmodule v1 = inr v2 ->
+  v1 ~~~ v2.
 Proof.
-  funelim (break_const_assigns_module_item mi).
-  all: clear Heqcall; simpl.
-  all: try LocationSet.setdec; expect 1.
-  funelim (break_const_assign target wf val).
-  all: simpl.
-  all: try LocationSet.setdec; expect 1.
-  rewrite module_body_writes_app.
-  rewrite H.
-  rewrite H0.
-  reflexivity.
+  unfold break_const_assigns_vmodule. simpl.
+  intros Hbreak.
+  monad_inv.
+  rename_match (vmodule_sorted v1) into Hsorted.
+  apply exact_by_output_equality.
+  intros initial.
+  unfold run_vmodule; simpl.
+  rewrite ! sort_module_items_stable.
+  - rewrite exec_break_const_assigns_module_body.
+    reflexivity.
+  - apply break_const_assigns_sorted.
+    exact Hsorted.
+  - exact Hsorted.
 Qed.
-
-From vera Require Import VerilogSemantics.
-Import ExactEquivalence.
-
-Lemma break_const_assign_width {w} (target : assign_target w) wf (val : XBV.xbv w) :
-  N_sum (map (fun '(AlwaysComb (@BlockingAssign w' _ _ _)) => w') (break_const_assign target wf val)) = w.
-Proof.
-  funelim (break_const_assign target wf val).
-  all: simpl; try apply N.add_0_r; expect 1.
-  rewrite map_app.
-  rewrite N_sum_app.
-  rewrite H.
-  rewrite H0.
-  reflexivity.
-Qed.
-
-Lemma break_const_assign_exes {w} (target : assign_target w) wf (val : BV.bitvector w) :
-  Forall
-    (fun mi =>
-      match mi with
-      | AlwaysComb (BlockingAssign lhs _ (IntegerLiteral _ val')) => exists bv_val', val' = XBV.from_bv bv_val'
-      | AlwaysComb (BlockingAssign lhs _ _) => True
-      end)
-    (break_const_assign target wf (XBV.from_bv val)).
-Proof.
-  revert val.
-  induction target.
-  all: intros.
-  all: simp break_const_assign.
-  all: eauto; expect 1.
-  apply Forall_app.
-  rewrite ! XBV.extr_no_exes by lia.
-  split.
-  - apply IHtarget1.
-  - apply IHtarget2.
-Qed.
-
-Theorem break_const_assigns_exact_equivalence {i o} (v : vmodule i o) :
-  break_const_assigns_vmodule v ~~~ v.
-Proof. Admitted.
